% Homework 1
% Minyoung Heo
% Jan 9 2024

# 2.8

$$
\ip{\bx}{\by}_2 = 2x_1 y_1 + 3x_2 y_1 + 3x_1 y_1 + 5x_2 y_2
$$

**1. Positivity**

$$
\begin{aligned}
\ip{\bx}{\bx}_2 = 2x_1 x_1 + 3x_1 x_2 + 3x_1 x_2 + 5x_2^2 \\
= 2x_1^2 + 6x_1 x_2 + 5x_2^2 \\
= 2(x_1^2 + 3x_1 x_2 + \frac{5}{2} x_2^2) \\
= 2(x_1^2 + 3x_1 x_2 + \frac{9}{4} x_2^2 + \frac{1}{4}x_2^2) \\
= 2(x_1 + \frac{3}{2}x_2)^2 + \frac{1}{2}x_2^2 \geq 0
\end{aligned} 
$$

It's easy to see that if $x=0$, then $\ip{\bx}{\bx}_2 = 0$

Now suppose $\ip{\bx}{\bx}_2 = 2(x_1 + \frac{3}{2}x_2)^2 + \frac{1}{2}x_2^2= 0$. That means

$2(x_1 + \frac{3}{2}x_2)^2 = -\frac{1}{2}x_2^2$ where $-\frac{1}{2}x_2^2 \leq 0$ and its equality is only when $x_2 = 0$.

Plugging it back in, $2(x_1 + \frac{3}{2}x_2)^2 \leq 0$ can only be true when $2(x_1 + \frac{3}{2}x_2^2)^2 = 0$ so $\bx = 0$

**2. Symmetry**

$$
\begin{aligned}
\ip{\bx}{\by}_2 = 2x_1 y_1 + 3x_2 y_1 + 3x_1 y_2 + 5x_2 y_2 \\
= 2y_1 x_1 + 3y_1 x_2 + 3y_2 x_1 + 5y_2 x_2 \\
= 2y_1 x_1 + 3y_2 x_1 + 3y_1 x_2 + 5y_2 x_2 \\
= \ip{\by}{\bx}_2
\end{aligned}
$$

**3. Additivity**

$$
\begin{aligned}
\ip{\bx+\by}{\bz}_2 = 2(x_1 + y_1) z_1 + 3(x_2 + y_2)z_1 + 3(x_1 + y_1)z_2 + 5(x_2 + y_2)z_2 \\
= 2x_1 z_2 + 3x_2 z_1 + 3x_1 z_2 + 5x_2 z_2 + 2y_1 z_1 + 3y_2 z_1 + 3y_1 z_2 + 5y_2 z_2 \\
= \ip{\bx}{\bz} + \ip{\by}{\bz}
\end{aligned}
$$

**4. Homogeneity**

$$
\begin{aligned}
\ip{r\bx}{\by} = 2(rx_1)y_1 + 3(rx_2)(y_1) + 3(rx_1)y_2 + 5(rx_2)y_2 \\
= r(2x_1 y_1 + 3x_2 y_1 + 3x_1 y_2 + 5x_2 y_2) \\
= r \ip{\bx}{\by}
\end{aligned}
$$

---

# 2.9

$$
\begin{aligned}
\bx = (\bx - \by) + \by \\
||\bx|| = ||(\bx - \by) + \by|| \leq ||\bx - \by|| + ||\by|| \\
\rightarrow ||\bx - \by|| \geq ||\bx|| - ||\by||
\end{aligned}
$$

But similarly, we can see that 

$$
||\by - \bx|| \geq ||\by|| - ||\bx||
$$

Since $||\by - \bx|| = ||\bx - \by||$, we can deduce that these are greater than the greater of the two, namely

$$
||\bx - \by|| \geq \mid ||\bx|| - ||\by|| \mid
$$



---

# 2.10

Since $||\bx - \by|| < \delta$,

$$
\left| ||\bx|| - ||\by|| \right| < \delta
$$
And we can let $\delta = \epsilon$.

---

# 3.8

$$
\begin{aligned}
A = \begin{bmatrix}
4 & -2 & 0 \\
2 & 1 & -1 \\
2 & -3 & 1
\end{bmatrix} = \begin{bmatrix}
4 & -2 & 0 \\
0 & 2 & -1 \\
0 & -2 & 1
\end{bmatrix} = \begin{bmatrix}
4 & -2 & 0 \\
0 & 2 & -1 \\
0 & 0 & 0
\end{bmatrix} = \begin{bmatrix}
4 & 0 & -1 \\
0 & 2 & -1 \\
0 & 0 & 0
\end{bmatrix}  \\
\end{aligned}
$$

$$
\begin{aligned}
2x_2 = x_3 \rightarrow x_2 = \frac{1}{2} x_3\\
4x_1 = x_3\rightarrow x_1 = \frac{1}{4}x_3 \\
\rightarrow N(A) = \text{span of } \Biggl\{ \begin{bmatrix} \frac{1}{2} \\ \frac{1}{4} \\ 1 \end{bmatrix} \Biggl\}
\end{aligned}
$$


---

# 3.9 

_**$R(A)$ is a subspace of $\R^m$**-:

**Existence of 0**:

$R(\mathbf{0}) = 0$ for any $m\times n$ zero matrix $\mathbf{0}$

**Closure under vector addition**:

Let $R(A)$ $\in$ $\mathbb{R}^m$ and $R(B) \in \mathbb{R}^m$ for $m \times n$ matrices $A$ and $B$.

For $R(A) + R(B) = \{Ax + By: x, y \in \R^m\}$, we can see that the span $\{Ax + By$ for any $x, y \in \R^m\}$ $\in \R^m$. Therefore, $R(A) + R(B) \in \R^m$ and thus the range is closed under vector addition.

**Closure under scalar multiplication**:

Let $R(A) \in \R^m$ and $\alpha \in \R$ for some $m \times n$ matrix A. 

$$
\alpha \cdot R(A) = \{\alpha Ax : x \in \R^n\}
$$
$\alpha A$ is still a $m \times n$ matrix and projects the $x$ onto the space $\R^m$. → $\alpha A x \in \R^m$ for any $x \in \R^n$ so $\alpha \cdot R(A) \in \R^m$ and thus the range is closed under scalar multiplication.

_**$N(A)$ is a subspace of $\R^n$**_:

**Existence of 0**:

$N(A)$ for some $n \times n$ matrix A such that its cols are linearly independent, $N(A) = 0$.

**Closure under vector addition**:

Let $N(A), N(B) \in \R^n$ for $m\times n$ matrices $A$ and $B$.

$$
N(A) + N(B) = \{x + y \in \R^n : Ax = 0, By = 0\} \\
$$

We can see that such vector $z = x + y \in \R^n$, thus $N(A) + N(B) \in \R^n$, and is closed under vector addition.

**Closure under scalar multiplication**

Let $N(A) \in R^n$ for some $m \times n$ matrix $A$ and $\alpha \in \R$.

$$
\alpha \cdot N(A) = \{\alpha x : A(\alpha x) = 0, x \in \R^n\}
$$
Both $x$ and $\alpha x$ are $\in \R^n$, so $\alpha \cdot N(A) \in \R^n$, so the nullspace is closed under scalar multiplication.

---

# 3.10

First we note that if we were to have $N(A^T) \subset N(B^T)$, we can deduce that

$$
N(B^T)^\perp \subset N(A^T)^\perp
$$

 (This is analogous to the following: suppose we have two sets $X$ and $Y$ and their respective complements $X^\prime$ and $Y^\prime$. If $X \subset Y$, then $Y^\prime \subset X^\prime$). 

Then we use **Theorem 3.4** (namely $R(A)^\perp = N(A^T)$ or equivalently $R(A) = N(A^T)^\perp$) to derive the conclusion

$$
R(B) \subset R(A)
$$



---

# 3.15

$$
\begin{aligned}
\begin{pmatrix}x_1 & x_2\end{pmatrix} \begin{bmatrix} 1 & -8 \\ 1 & 1 \end{bmatrix} \begin{pmatrix} x_1 \\ x_2\end{pmatrix} \\
= \begin{bmatrix}x_1 + x_2 & -8x_1 + x_2 \end{bmatrix} \begin{pmatrix} x_1 \\ x_2 \end{pmatrix} \\
= x_1^2 + x_1 x_2 - 8x_1 x_2 + x_2^2 \\
= x_1^2 - 7x_1 x_2 + x_2^2 \quad (\text{Use this one for calculations})\\
= x_1^2 - 7x_1 x_2 + \frac{49}{4}x_2^2 - \frac{45}{4}x_2^2 \\
= (x_1 - \frac{7}{2}x_2)^2 - \frac{45}{4}x_2^2
\end{aligned}
$$

All we need to do is first check for cases where $(x_1 - \frac{7}{2}x_2)^2 - \frac{45}{4}x_2^2 < 0$ and then check for $(x_1 - \frac{7}{2}x_2)^2 - \frac{45}{4}x_2^2 > 0$.

For $(x_1 - \frac{7}{2}x_2)^2 - \frac{45}{4}x_2^2 < 0$ :

$$
\begin{aligned}
(x_1-\frac{7}{2}x_2)^2 < \frac{45}{4} x^2, \text{so } \\
-\sqrt{\frac{45}{4}}x_2 < x_1 - \frac{7}{2}x_2 < \sqrt{\frac{45}{4}}x_2 \\
\rightarrow \frac{7-\sqrt{45}}{2}x_2 < x_1 < \frac{7+\sqrt{45}}{2}x_2
\end{aligned}
$$

An example of this is when $x_1 = \frac{7}{2}x_2$ → $x = \begin{pmatrix}\frac{7}{2} \\ 1\end{pmatrix}$. Plugging this into $x_1^2 - 7x_1 x_2 + x_2^2$, we get $-\frac{45}{4} < 0$.

For $(x_1 - \frac{7}{2}x_2)^2 - \frac{45}{4}x_2^2 > 0$ :

$$
\begin{aligned}
(x_1-\frac{7}{2}x_2)^2 > \frac{45}{4} x^2, \text{so } \\
x_1 - \frac{7}{2}x_2 < -\sqrt{\frac{45}{4}}x_2 \cup x_1 - \frac{7}{2}x_2 > \sqrt{\frac{45}{4}}x_2 \\
\rightarrow x_1 < \frac{7-\sqrt{45}}{2}x_2 \cup x_1 > \frac{7+\sqrt{45}}{2}x_2
\end{aligned}
$$

An example of this is when $x_1 = \frac{100}{2}x_2$ → $x = \begin{pmatrix}\frac{100}{2} \\ 1\end{pmatrix}$. Plugging this into $x_1^2 - 7x_1 x_2 + x_2^2$, we get $9301 > 0$.

Therefore this is **indefinite**.

---

# 3.16

$$
\begin{aligned}
\Delta_1 = 2 \\
\Delta_2 = \begin{vmatrix} 2 & 2 \\ 2&2 \end{vmatrix} = 0\\
\Delta_3 = \begin{vmatrix} 2 & 2 & 2 \\ 2& 2& 2 \\2&2&0\end{vmatrix} = 2\begin{vmatrix}2&2\\2&0\end{vmatrix} - 2\begin{vmatrix}2&2\\2&0\end{vmatrix} + 2\begin{vmatrix}2&2\\2&2\end{vmatrix} = 2\begin{vmatrix}2&2\\2&2\end{vmatrix} = 0
\end{aligned}
$$

And all of them are nonnegative.

Looking at the quadratic form $x^T \begin{bmatrix}2 & 2 & 2\\2&2&2\\2&2&0\end{bmatrix} x$:

$$
\begin{aligned}
x^T \begin{bmatrix}2 & 2 & 2\\2&2&2\\2&2&0\end{bmatrix} x  =\begin{bmatrix}2x_1+2x_2+2x_3 & 2x_1 + 2x_2+2x_3 & 2x_1 + 2x_2 \end{bmatrix}\begin{bmatrix}x_1\\x_2\\x_3\end{bmatrix} \\
= 2x_1^2 + 2x_1x_2 + 2x_1x_3 + 2x_1x_2 + 2x_2^2 + 2x_2x_3 + 2x_1x_3 + 2x_2x_3 \\
= 2x_1^2 + 2x_2^2 + 4x_1x_2 + 4x_1x_3 + 4x_2x_3 \\
= 2(x_1 + x_2)^2 + 4x_3(x_1 + x_2)
\end{aligned}
$$

Now we try to make $x_1 + x_2 < -2x_3$, while making sure $|x_1 + x_2| < |2x_3|$. So by setting $x_3 = 1$, we can easily produce an example vector $x = \begin{bmatrix}-\frac{1}{10} \\ -\frac{1}{10} \\ 1\end{bmatrix}$. If we plug this back into $2(x_1 + x_2)^2 + 4x_3(x_1 + x_2)$, we get 

$$
2(-0.2)^2 + 4(1)(0.2) = 0.08 - 0.8 < 0
$$

As we can see, there exists a vector such that it's not positive definite, so $A$ is not positive definite.