% Homework 2
% Math 436
% Minyoung Heo

# 3.17

## a)

$\text{det}(Q - \lambda I) = \begin{vmatrix}-\lambda&1&1\\1&-\lambda&1\\1&1&-\lambda\end{vmatrix}$

$$
\begin{aligned}
= -\lambda \begin{vmatrix}-\lambda&1\\1&-\lambda\end{vmatrix} - 1 \begin{bmatrix}1&1\\1&-\lambda\end{bmatrix} + 1 \begin{vmatrix}1&-\lambda\\1&-\lambda\end{vmatrix}\\
= -\lambda^2(\lambda^2 - 1) - 1(-\lambda-1) + (1 + \lambda) \\
= -\lambda^3 + \lambda + 2\lambda + 2 \\
= -\lambda^3 +3\lambda + 2\\
\rightarrow \lambda^3 - 3\lambda - 2 = 0
\end{aligned}
$$
By using Zero Remainder Theorem, we can deduce that -1 is a root so, doing some long division (not in this sheet)

$$
\lambda^3-3\lambda-2 = (\lambda+1)^2(\lambda-2) = 0
$$

Which we can see since $\lambda = -1, 2$, this is **indefinite**.

## b)

Computing the eigenvectors, for $\lambda_1 = -1$

$$
\begin{amatrix}{3}
1 & 1 & 1 & 0 \\
1 & 1 & 1 & 0\\
1 & 1 & 1& 0
\end{amatrix} \rightarrow
v_1 = \begin{bmatrix}-1\\1\\0 \end{bmatrix} x_2 + \begin{bmatrix}-1\\0\\1\end{bmatrix}x_3
$$
And for $\lambda_2 = 2$

$$
\begin{aligned}
\begin{amatrix}{3}
-2 & 1 & 1 & 0 \\
1 & -2 & 1 & 0\\
1 & 1 & -2& 0
\end{amatrix} \rightarrow
\begin{amatrix}{3}
-2 & 1 & 1 & 0 \\
0 & -\frac{3}{2} & \frac{3}{2} & 0\\
0 & \frac{3}{2} & -\frac{3}{2} & 0
\end{amatrix} \rightarrow
\begin{amatrix}{3}
-2 & 1 & 1 & 0 \\
0 & 1 & -1 & 0\\
0 & -1 & 1 & 0
\end{amatrix}\\ \rightarrow
x_2 = x_3; 2x_1 = x_2 + x_3 \rightarrow
v_2 = \begin{bmatrix}1\\1\\1 \end{bmatrix}
\end{aligned}
$$
We can see that for $v_2 \not\in M$. In fact $v_1$ spans $M$ so we get that $v_2$ is orthogonal to $M$. We can disregard the eigenvalue $\lambda_2$, so we get that Q is negative definite.e



---

# 3.22

Frist we note that 

$$
\begin{aligned}
||A||_\infty = \max_{||x||_\infty = 1} ||Ax||_\infty \\
= \max_{||x||=1} || \sum_{j=1}^n A_j x_j||_\infty \quad (\text{where } A_j \text{is the }j\text{th column of }A)\\
= \max_{||x||_\infty=1} \left( \max_{1\leq i\leq n} \left| \sum_{j=1}^n A_j x_j\right| \right) 
\end{aligned}
$$

As a kind of illustration, we can see 

$$
||Ax||_\infty = \max_{1\leq j\leq n} \left[\begin{pmatrix}a_{11}\\a_{21}\\...\\a_{m1}\end{pmatrix}x_1 + \begin{pmatrix}a_{12}\\a_{22}\\...\\a_{m2}\end{pmatrix}x_2 + … + \begin{pmatrix}a_{1n}\\a_{2n}\\...\\a_{mn}\end{pmatrix}x_n \right]
$$

If $||x||_\infty = 1$, we can maximize each $x_j$ to be $\pm 1$ such that the maximum row sum can be made. Thus we can make

$$
\max_{||x||_\infty=1} \left( \max_{1\leq i\leq n} \left| \sum_{j=1}^n A_j x_j\right| \right) = \max_{1\leq i \leq n} \sum_{j=1}^n |A_{ij}|
$$

---

# 5.3

## a)

If we write $f(x) = (a^Tx)(b^Tx) = (a_1x_1 + … + a_nx_n)(b_1x_1 + … + b_nx_n)$, we can calculate each partial derivative. 

$$
\begin{aligned}
\frac{\partial f}{\partial x_1} = a_1 (b_1x_1 + … + b_nx_n) + b_1(a_1 x_1 + … + a_n x_n) \\
= a_1(b^Tx) + b_1(a^Tx) \\
... \\
\frac{\partial f}{\partial x_k} = a_k (b^Tx) + b_k(a^Tx)
\end{aligned}
$$

And that gives us the gradient:

$$
\nabla f(x) = \begin{bmatrix} a_1(b^Tx) + b_1(a^Tx) \\ .\\.\\. \\ a_k (b^Tx) + b_k(a^Tx) \\ .\\.\\. \\ a_n(b^Tx) + b_n(a^Tx) \end{bmatrix}
$$

## b)

If we take each $k$th term: $\frac{\partial f}{\partial x_k} = a_k (b_1x_1 + … + b_nx_n) + b_k(a_1x_1 + … + a_nx_n)$, we can treat $k$ as the "row" and $l$ as the "column" for the Jacobian:

$$
\begin{aligned}
\frac{\partial f}{\partial x_k}=a_k(b_1x_1+...+b_nx_n) + b_k(a_1x_1+...+a_nx_n) \\
\frac{\partial^2 f}{\partial x_l \partial x_k} = a_kb_l + b_ka_l\\
\rightarrow D^2 f = \begin{bmatrix}2a_1b_1 & a_1b_1 + b_1a_1 & … & a_1b_n + b_1a_n \\ 
. & . & . & . \\
. & . & . & . \\
. & . & . & . \\
a_nb_1 + b_na_1 & a_nb_2 + b_na_2 & … & 2a_nb_n \end{bmatrix}
\end{aligned}
$$

---

# 5.6

Let $f(x(t)) = (e^t + t^3)^3t^2(t+1)^2 + (e^t + t^3)t^2 + t + 1$. 

$$
\begin{aligned}
\frac{d}{dt} f(x(t)) = 3(e^t+t^3)^2t^2(t+1)^2(e^t + 3t^2) + (e^t+t^3)^3(2t)(t+1)^2 \\
						+ (e^t+t^3)^3t^2(2(t+1)) + (e^t+3t^2)(t^2) + (e^t + t^3)(2t) + 1
\end{aligned}
$$


With a bit of simplification:

$$
= (e^t+t^3)^3[4t^3 + 6t^2 + 2t ] + t^2(e^t+3t^2)[3(e^t + t^3)^2t^2(t+1)^2 + 1] + (e^t+t^3)2t + 1
$$

---

# 5.10

## a) 

$$
\begin{aligned}
f(x_0) = 1 + 1 = 2 \\
f^\prime(x_0) = \left[\frac{\partial f}{\partial x_1} \quad \frac{\partial f}{\partial x_2} \right] = [e^{-x_2} \quad -x_1e^{-x_2}+1] \\
		= [1 \quad 0] \\
f^{\prime \prime}(x_0) = \begin{bmatrix}\frac{\partial^2 f}{\partial x_1^2} & \frac{\partial^2 f}{\partial x_1x_2} \\ \frac{\partial^2 f}{\partial x_2x_1} & \frac{\partial^2 f}{\partial x_2^2} \end{bmatrix} = \begin{bmatrix} 0 & -e^{-x_2} \\ -e^{-x_2} & x_1e^{-x_2} \end{bmatrix} \\
		= \begin{bmatrix}0 & -1 \\ -1 & 1\end{bmatrix}
\end{aligned}
$$

With all of these calculated, we can get the taylor's expansion:

$$
\begin{aligned}
f(x) = 2 + [1 \quad 0] \begin{bmatrix}x_1-1\\x_2\end{bmatrix} + \frac{1}{2}\begin{bmatrix}x_1-1&x_2\end{bmatrix} \begin{bmatrix}0&-1\\-1&1\end{bmatrix} \begin{bmatrix}x_1-1\\x_2\end{bmatrix}  \\ 
= 2 + x_1 - 1 + \frac{1}{2}\begin{bmatrix}-x_2&-x_1+1+x_2\end{bmatrix} \begin{bmatrix}x_1-1\\x_2\end{bmatrix} \\
=1 + x_1 + \frac{1}{2}(-x_1x_2 + x_2 - x_1x_2 + x_2 + x_2^2) \\
= 1 + x_1 + \frac{1}{2}x_2^2 + x_2 - x_1 x_2
\end{aligned}
$$

## b)

$$
\begin{aligned}
f(x_0) = 1 +2+ 1 = 4 \\
f^\prime(x_0) = \left[\frac{\partial f}{\partial x_1} \quad \frac{\partial f}{\partial x_2} \right] = [3x_1^3 + 4x_1x_2^2 \quad 4x_1^2x_2 + 3x_2^3] \\
		= [7 \quad 7] \\
f^{\prime \prime}(x_0) = \begin{bmatrix}\frac{\partial^2 f}{\partial x_1^2} & \frac{\partial^2 f}{\partial x_1x_2} \\ \frac{\partial^2 f}{\partial x_2x_1} & \frac{\partial^2 f}{\partial x_2^2} \end{bmatrix} = \begin{bmatrix} 9x_1^2 + 4x_2^2 & 8x_1x_2\\ 8x_1x_2 & 4x_1^2+9x_2^2 \end{bmatrix} \\
		= \begin{bmatrix}13 & 8 \\ 8 & 13\end{bmatrix}
\end{aligned}
$$

With all of these calculated, we can get the taylor's expansion:

$$
\begin{aligned}
f(x) = 4 + [7 \quad 7] \begin{bmatrix}x_1-1\\x_2-1\end{bmatrix} + \frac{1}{2}\begin{bmatrix}x_1-1&x_2-1\end{bmatrix} \begin{bmatrix}13&8\\8&13\end{bmatrix} \begin{bmatrix}x_1-1\\x_2-1\end{bmatrix}  \\ 
= 4 + 7x_1 - 7 + 7x_2-7 + \frac{1}{2}\begin{bmatrix}13x_1-13+8x_2-8&8x_1-8+13x_2-13\end{bmatrix} \begin{bmatrix}x_1-1\\x_2-1\end{bmatrix} \\
=-10 + 7x_1 + 7x_2 + \frac{1}{2}((13x_1 + 8x_2 -21)(x_1-1) + (8x_1+13x_2-21)(x_2-1)) \\
=-10 + 7x_1 + 7x_2 + \frac{1}{2}(13x_1^2+13x_2^2+16x_1x_2-42x_1-42x_2+42) \\
= 11 - 14x_1-14x_2+8x_1x_2 + \frac{13}{2}x_1^2 + \frac{13}{2}x_2^2
\end{aligned}
$$

## c)

$$
\begin{aligned}
f(x_0) = e + 1 + e + 1 = 2e + 2 \\
f^\prime(x_0) = \left[\frac{\partial f}{\partial x_1} \quad \frac{\partial f}{\partial x_2} \right] = [e^{x_1-x_2} + e^{x_1+x_2}+1 \quad -e^{x_1-x_2} + e^{x_1+x_2}+1] \\
		= [e+e+1 \quad -e+e+1] = [2e+1 \quad 1] \\
f^{\prime \prime}(x_0) = \begin{bmatrix}\frac{\partial^2 f}{\partial x_1^2} & \frac{\partial^2 f}{\partial x_1x_2} \\ \frac{\partial^2 f}{\partial x_2x_1} & \frac{\partial^2 f}{\partial x_2^2} \end{bmatrix} = \begin{bmatrix} e^{x_1-x_2}+e^{x_1+x_2} & -e^{x_1-x_2}+e^{x_1+x_2} \\ -e^{x_1-x_2}+e^{x_1+x_2} & e^{x_1-x_2}+e^{x_1+x_2} \end{bmatrix} \\
		= \begin{bmatrix}e+e & -e+e \\ -e+e & e+e\end{bmatrix} = \begin{bmatrix}2e & 0 \\ 0 & 2e\end{bmatrix}
\end{aligned}
$$

With all of these calculated, we can get the taylor's expansion:

$$
\begin{aligned}
f(x) = 2e+2 + [2e+1 \quad 1] \begin{bmatrix}x_1-1\\x_2\end{bmatrix} + \frac{1}{2}\begin{bmatrix}x_1-1&x_2\end{bmatrix} \begin{bmatrix}2e&0\\0&2e\end{bmatrix} \begin{bmatrix}x_1-1\\x_2\end{bmatrix}  \\ 
= 2e + 2 + (2e+1)x_2-2e-1 + x_2 + \frac{1}{2}\begin{bmatrix}2e(x_1-1)&2ex_2\end{bmatrix} \begin{bmatrix}x_1-1\\x_2\end{bmatrix} \\
=1+(2e+1)x_1 + x_2 + e((x_1-1)^2+x_2^2) \\
= 1+(2e+1)x_1 + x_2 +ex_1^2 -2ex_1 + e + ex_2^2 \\
= 1+e+x_1+x_2+e(x_1^2 + x_2^e)
\end{aligned}
$$



---
